\documentclass{article}
\usepackage{xcolor}
\input{../../../../recursos/latex/Algo1Macros.tex}

\begin{document}

\section*{Ejercicio 5}

\subsection*{a)}

\begin{verbatim}
    j:= 1;
    result:= 0;
    while(j < s.size()) do
        if j mod 2 = 1 then result:= result + s[j]; else skip; fi;
        j:= j + 1;
    endwhile
\end{verbatim}

\subsection*{Teorema del invariante}
\begin{itemize}
    \item $P_{c} \implica I$
    \item $(I \wedge \neg B) \implica Q_{c}$
    \item $\{I \wedge B\}$ ciclo $\{ I \}$
    \item $\{I \wedge B \wedge (v_{0} = f_{v})\}$ ciclo $\{f_{v} < v_{0}\}$
    \item $(I \wedge f_{v} \leq 0) \implica \neg B$
\end{itemize}


\subsection*{DemostraciÃ³n}
\subsubsection*{Datos}
\begin{itemize}
    \item $P_{c}    \equiv j = 1 \wedge result = 0$
    \item $Q_{c}    \equiv result = \sum_{i=0}^{\longitud{s}-1} \IfThenElse{i \bmod 2 = 1}{s[i]}{0}$
    \item $I        \equiv 0 \leq j \leq \longitud{s} \yLuego result = \sum_{i=0}^{j-1} \IfThenElse{i \bmod 2 = 1}{s[i]}{0}$
    \item $B        \equiv j < \longitud{s}$
    \item $S1       \equiv \IfThenElse{j \bmod 2 = 1}{result:= result + s[j];}{skip;}$
    \item $S2       \equiv j:= j + 1;$
    \item $ciclo    \equiv S1;S2;$
    \item $f_{v}    \equiv \longitud{s}-j$
\end{itemize}

\subsubsection*{$P_{c} \implica I$}

$P_{c} \implica I \equiv$

$j = 1 \wedge result = 0 \implica$
$0 \leq j \leq \longitud{s} \yLuego result = \sum_{i=0}^{j-1} \IfThenElse{i \bmod 2 = 1}{s[i]}{0}$

\begin{itemize}
    \item $j = 1 \wedge result = 0 \implica 0 \leq j \leq \longitud{s} \yLuego result = \sum_{i=0}^{j-1} \IfThenElse{i \bmod 2 = 1}{s[i]}{0} \equiv \True$
\end{itemize}

\subsubsection*{$(I \wedge \neg B) \implica Q_{c}$}

$(I \wedge \neg B) \implica Q_{c} \equiv$

$0 \leq j \leq \longitud{s} \yLuego result = \sum_{i=0}^{j-1} \IfThenElse{i \bmod 2 = 1}{s[i]}{0} \wedge j \geq \longitud{s} \implica$
$result = \sum_{i=0}^{\longitud{s}-1} \IfThenElse{i \bmod 2 = 1}{s[i]}{0} \equiv$

$j = \longitud{s} \yLuego result = \sum_{i=0}^{j-1} \IfThenElse{i \bmod 2 = 1}{s[i]}{0} \implica$
$result = \sum_{i=0}^{\longitud{s}-1} \IfThenElse{i \bmod 2 = 1}{s[i]}{0} \equiv \True$

\subsubsection*{$\{I \wedge B\}$ ciclo $\{ I \}$}

$wp(S1;S2, I) \stackrel{Ax3}{\equiv}$

$wp(S1, wp(S2, I))$

\begin{itemize}
    \item $wp(S2; I) \equiv$

    $wp(j:= j+1, 0 \leq j \leq \longitud{s} \yLuego result = \sum_{i=0}^{j-1} \IfThenElse{i \bmod 2 = 1}{s[i]}{0}) \stackrel{Ax4}{\equiv}$

    $\{0 \leq j+1 \leq \longitud{s} \yLuego result = \sum_{i=0}^{j+1} \IfThenElse{i \bmod 2 = 1}{s[i]}{0} \}$

    \item $wp(S1, wp(S2, I)) \equiv$

    $wp(\IfThenElse{j \bmod 2 = 1}{result:= result + s[j];}{skip;},0 \leq j+1 \leq \longitud{s} \yLuego result = \sum_{i=0}^{j} \IfThenElse{i \bmod 2 = 1}{s[i]}{0})\equiv$\\

    $\{ ((j \bmod 2 = 1) \wedge wp(result:=result + s[j], 0 \leq j+1 \leq \longitud{s} \yLuego result = \sum_{i=0}^{j} \IfThenElse{i \bmod 2 = 1}{s[i]}{0}) \vee $

    $ (j \bmod 2 \neq 1) \wedge wp(skip, 0 \leq j+2 \leq \longitud{s} \yLuego result = \sum_{i=0}^{j} \IfThenElse{i \bmod 2 = 1}{s[i]}{0}))\} \equiv$\\

    $\{ ((j \bmod 2 = 1) \wedge 0 \leq j < \longitud{s} \yLuego (0 \leq j+2 \leq \longitud{s} \yLuego result + s[j] = \sum_{i=0}^{j} \IfThenElse{i \bmod 2 = 1}{s[i]}{0}) \vee $

    $ (j \bmod 2 \neq 1) \wedge (0 \leq j+1 \leq \longitud{s} \yLuego result = \sum_{i=0}^{j+1} \IfThenElse{i \bmod 2 = 1}{s[i]}{0}))\} \equiv$\\

    $\{ ((j \bmod 2 = 1) \wedge (0 \leq j < \longitud{s} \yLuego result + s[j] = \sum_{i=0}^{j+1} \IfThenElse{i \bmod 2 = 1}{s[i]}{0}) \vee $

    $ (j \bmod 2 \neq 1) \wedge (0 \leq j+1 \leq \longitud{s} \yLuego result = \sum_{i=0}^{j+1} \IfThenElse{i \bmod 2 = 1}{s[i]}{0}))\}$

\end{itemize}

Qvq $I \wedge B \implica wp(S1;S2, I)$

\begin{itemize}
    \item $I \wedge B \equiv$
    
    $0 \leq j \leq \longitud{s} \yLuego result = \sum_{i=0}^{j-1} \IfThenElse{i \bmod 2 = 1}{s[i]}{0} \wedge j < \longitud{s} \equiv$

    $0 \leq j < \longitud{s} \yLuego result = \sum_{i=0}^{j-1} \IfThenElse{i \bmod 2 = 1}{s[i]}{0} \equiv$

    \item $I \wedge B \implica wp(S1;S2, I) \equiv$

    $0 \leq j < \longitud{s} \yLuego result = \sum_{i=0}^{j-1} \IfThenElse{i \bmod 2 = 1}{s[i]}{0} \implica$

    $((j \bmod 2 = 1) \wedge (0 \leq j < \longitud{s} \yLuego result + s[j] = \sum_{i=0}^{j} \IfThenElse{i \bmod 2 = 1}{s[i]}{0}) \vee $

    $ (j \bmod 2 \neq 1) \wedge (0 \leq j+1 \leq \longitud{s} \yLuego result = \sum_{i=0}^{j} \IfThenElse{i \bmod 2 = 1}{s[i]}{0})) \equiv \True$

\end{itemize}

\subsubsection*{$\{I \wedge B \wedge (v_{0} = f_{v})\}$ ciclo $\{f_{v} < v_{0}\}$}

$wp(S1;S2, \longitud{s}-j<v_{0}) \stackrel{Ax3}{\equiv}$

$wp(S1, wp(S2, \longitud{s}-j<v_{0})) \stackrel{Ax3}{\equiv}$

\begin{itemize}
    \item $wp(S2, n-i<v_{0}) \equiv$
    
    $ wp(j:= j+1, \longitud{s}-j<v_{0})) \stackrel{Ax1}{\equiv}$

    $\{\longitud{s}-j-1<v_{0}) \}$

    \item $wp(S1, wp(S2, f_{v} < v_{0})) \equiv$

    $wp(\IfThenElse{j \bmod 2 = 1}{result:= result + s[j];}{skip;}, \longitud{s}-j-1<v_{0}) \stackrel{Ax4}{\equiv}$

    $\{(j \bmod 2 = 1) \wedge (0 \leq j < \longitud{s} \yLuego \longitud{s}-j-1<v_{0}) \vee $

    $ (j \bmod 2 \neq 1) \wedge \longitud{s}-j-1<v_{0}\}$

\end{itemize}

Qvq $(I \wedge B \wedge (v_{0} = f_{v})) \implica wp(S1;S2, f_{v} < v_{0})$ \\

$(I \wedge B \wedge (v_{0} = f_{v})) \implica wp(S1;S2, f_{v} < v_{0}) \equiv$ \\

$0 \leq j < \longitud{s} \yLuego result = \sum_{i=0}^{j-1} \IfThenElse{i \bmod 2 = 1}{s[i]}{0} \wedge (v_{0} = \longitud{s}-j)\implica$

$((j \bmod 2 = 1) \wedge (0 \leq j < \longitud{s} \yLuego \longitud{s}-j-1<v_{0})) \vee ((j \bmod 2 \neq 1) \wedge ()\longitud{s}-j-1<v_{0})) \equiv \True$

\subsubsection*{$(I \wedge f_{v} \leq 0) \implica \neg B$}

$(I \wedge f_{v} \leq 0) \implica \neg B \equiv $

$0 \leq j \leq \longitud{s} \yLuego result = \sum_{i=0}^{j-1} \IfThenElse{i \bmod 2 = 1}{s[i]}{0} \wedge \longitud{s}-j \leq 0 \implica j \geq \longitud{s} $

$\equiv \True$

\end{document}