
\begin{proc}{reconstruir}{\In $s$: $se\tilde{n}al$,
    \In $prof$: \ent,
    \In $freq$: \ent,
    \Out $result$: $se\tilde{n}al$}{}
\pre{ esSe\tilde{n}alAux(s, prof, freq) \wedge tieneAlMenos2MuestrasDistintasDeCero(s) }
\post{

    $\quad \longitud{s} = \longitud{result}\ \yLuego ($

        $\quad\quad enDondeNoSeaCeroDebenCoincidir(s, result)\ \wedge$

        $\quad\quad enDondeEsCeroDebeSerElPromedioDeSusVecinosNoNulos(s, result))$

}
\end{proc}

\pred{tieneAlMenos2MuestrasDistintasDeCero}{s: se√±al}{
    (\longitud{s} - \#apariciones(s, 0)) \geq 2
}

$ $

\pred{enDondeNoSeaCeroDebenCoincidir}{$original$: $se\tilde{n}al$,
    $reconstruida$: $se\tilde{n}al$}
{

    $\quad\paraTodo{i}{0}{\longitud{original}}$
    $\implicaLuego$
    $((original[i] \neq 0) \implica (original[i] = reconstruida[i]))$

}

$ $

\pred{enDondeEsCeroDebeSerElPromedioDeSusVecinosNoNulos}{$original$: $se\tilde{n}al$,
    $reconstruida$: $se\tilde{n}al$}
{

    $\quad\paraTodo{i}{0}{\longitud{original}}$
    $\implicaLuego$
    $((original[i] = 0) \implica $

    $\quad\quad esUnPromedioDeSusVecinosNoNulosMasCercanos(original, reconstruida, i))$

}

$ $

\pred{esUnPromedioDeSusVecinosNoNulosMasCercanos}{$original$:$se\tilde{n}al$,
$reconstruida$:$se\tilde{n}al$,
$i$: \ent}{

    $\quad \existe{j,k,l}{0}{\longitud{original}} \wedge $
    $(dist(j, i) < dist(i, k) \wedge dist(j, i) < dist(i, l)) \yLuego ($

        $\quad\quad (s[j] \neq 0 \wedge s[k] \neq 0 \wedge s[l] \neq 0)\ \wedge$

        $\quad\quad ($
        $ \paraTodo{m}{0}{\longitud{original}} \wedge m \notin [i, j, k, l] \implicaLuego $

        $\quad\quad\quad\quad original[m] \neq 0\ \implica $

        $\quad\quad\quad\quad ($
            $dist(i, m) \geq dist(i, j)\ \wedge$
            $dist(i, m) \geq dist(i, k)\ \wedge $
            $dist(i, m) \geq dist(i, l)$
            $)$
        $)\ \wedge$

        $\quad\quad($
            $reconstruida[i] \in [promedio(original[j],original[k]), promedio(original[j],original[l])]$
        $)$
    $)$

}

$ $

\aux{dist}{$x$: \ent,
    $y$: \ent}{\ent}{
    abs(x-y)
}

$ $

\aux{promedio}{$a$: \ent,
    $b$: \ent}{\ent}{
    (a+b)\ div\ 2
}
