\documentclass{article}
\usepackage{xcolor}
\input{../../../../recursos/latex/Algo1Macros.tex}

\begin{document}

\section*{Ejercicio 11}

\subsection*{Correctitud}
\begin{itemize}
    \item $Pre \implica wp($codigo previo al ciclo$, P_{c})$
    \item $P_{c} \implica wp(ciclo, Q_{c})$
    \item $Q_{c} \implica wp($codigo posterior al ciclo$, Post)$
\end{itemize}

Por monotonía sabemos que Pre \implica wp(programa completo, Post)

\subsection*{Teorema del invariante}
\begin{itemize}
    \item $P_{c} \implica I$
    \item $(I \wedge \neg B) \implica Q_{c}$
    \item $\{I \wedge B\}$ ciclo $\{ I \}$
    \item $\{I \wedge B \wedge (v_{0} = f_{v})\}$ ciclo $\{f_{v} < v_{0}\}$
    \item $(I \wedge f_{v} \leq 0) \implica \neg B$
\end{itemize}

\subsection*{Demostración}

\subsubsection*{Datos}
\begin{itemize}
    \item $Pre      \equiv \True$
    \item $Post     \equiv r = -1 \implica \paraTodo{j}{(0}{\longitud{s}} \implicaLuego s[j] \neq e) \wedge r \neq -1 \implica (0 \leq r < \longitud{s}\yLuego s[r]=e)$
    \item $P_{c}    \equiv i = (\longitud{s} - 1) \wedge j = -1 $
    \item $Q_{c}    \equiv j = -1 \implica \paraTodo{j}{(0}{\longitud{s}} \implicaLuego s[j] \neq e) \wedge j \neq -1 \implica (0 \leq j < \longitud{s}\yLuego s[j]=e)$
    \item $I        \equiv 0 \leq i < \longitud{s} \yLuego j = -1 \implica \paraTodo{j}{(i+1}{\longitud{s}} \implicaLuego s[j] \neq e) \wedge j \neq -1 \implica (i < j < \longitud{s} \yLuego s[j]=e)$
    \item $B        \equiv i \geq 0$
    \item $S1       \equiv \IfThenElse{s[i]=e}{j:=i}{skip}$
    \item $S2       \equiv i:= i - 1$
    \item $ciclo    \equiv S1;S2;$
    \item $f_{v}    \equiv i$
\end{itemize}

\subsubsection*{$Pre \implica wp($codigo previo al ciclo$, P_{c})$}

$wp($codigo previo al ciclo$, P_{c}) \equiv$

$wp(i:= \longitud{s}-1;j:= -1, i = (\longitud{s} - 1) \wedge j = -1) \stackrel{Ax3}{\equiv}$

$wp(i:= \longitud{s}-1, wp(j:= -1, i = (\longitud{s} - 1) \wedge j = -1) $

\begin{itemize}
    \item $wp(j:= -1, i = (\longitud{s} - 1) \wedge j = -1)\stackrel{Ax1}{\equiv}$

    $ \{ i = (\longitud{s} - 1) \wedge -1 = -1 \} $
\end{itemize}

$wp(i:= \longitud{s}-1, i = (\longitud{s} - 1) \wedge -1 = -1) \stackrel{Ax1}{\equiv}$

$ \longitud{s} -1 = \longitud{s} - 1 \wedge -1 = -1 \equiv \True $

$Pre \implica wp($codigo previo al ciclo$, P_{c}) \equiv$

$\True \implica \True \equiv \True$

\subsubsection*{$Q_{c} \implica wp($codigo posterior al ciclo$, Post)$}

$wp($codigo posterior al ciclo$, Post) \equiv$

$wp(r:= j, r = -1 \implica \paraTodo{j}{(0}{\longitud{s}} \implicaLuego s[j] \neq e) \wedge r \neq -1 \implica (0 \leq r < \longitud{s}\yLuego s[r]=e) \equiv$

$\{ j = -1 \implica \paraTodo{j}{(0}{\longitud{s}} \implicaLuego s[j] \neq e) \wedge r \neq -1 \implica (0 \leq j < \longitud{s}\yLuego s[j]=e \}$

$Q_{c} \implica wp($codigo posterior al ciclo$, Post \equiv$

$j = -1 \implica \paraTodo{j}{(0}{\longitud{s}} \implicaLuego s[j] \neq e) \wedge j \neq -1 \implica (0 \leq j < \longitud{s}\yLuego s[j]=e) \implica$

$j = -1 \implica \paraTodo{j}{(0}{\longitud{s}} \implicaLuego s[j] \neq e) \wedge r \neq -1 \implica (0 \leq j < \longitud{s}\yLuego s[j]=e \equiv \True$

\subsubsection*{$P_{c} \implica wp(ciclo, Q_{c})$}

\begin{itemize}
    \item $P_{c} \implica I$
    $i = (\longitud{s} - 1) \wedge j = -1 \implica$

    $0 \leq i < \longitud{s} \yLuego j = -1 \implica \paraTodo{j}{(i+1}{\longitud{s}} \implicaLuego s[j] \neq e) \wedge j \neq -1 \implica (i < j < \longitud{s} \yLuego s[j]=e) \equiv \True$

    \item $(I \wedge \neg B) \implica Q_{c}$
    
    $0 \leq i < \longitud{s} \yLuego j = -1 \implica \paraTodo{j}{(i+1}{\longitud{s}} \implicaLuego s[j] \neq e) \wedge j \neq -1 \implica (i < j < \longitud{s} \yLuego s[j]=e) \wedge i < 0 \implica$

    $j = -1 \implica \paraTodo{j}{(0}{\longitud{s}} \implicaLuego s[j] \neq e) \wedge j \neq -1 \implica (0 \leq j < \longitud{s}\yLuego s[j]=e) \equiv$

    $\False \implica j = -1 \implica \paraTodo{j}{(0}{\longitud{s}} \implicaLuego s[j] \neq e) \wedge j \neq -1 \implica (0 \leq j < \longitud{s}\yLuego s[j]=e) \equiv \True$

    \item $\{I \wedge B\}$ ciclo $\{ I \}$
    
    $wp(i:i-1, 0 \leq i < \longitud{s} \yLuego j = -1 \implica \paraTodo{j}{(i+1}{\longitud{s}} \implicaLuego s[j] \neq e) \wedge j \neq -1 \implica (i < j < \longitud{s} \yLuego s[j]=e))\equiv$

    $0 \leq i-1 < \longitud{s} \yLuego j = -1 \implica \paraTodo{j}{(i}{\longitud{s}} \implicaLuego s[j] \neq e) \wedge j \neq -1 \implica (i-1 < j < \longitud{s} \yLuego s[j]=e)$

    $wp(\IfThenElse{s[i]=e}{j:=i}{skip},0 \leq i-1 < \longitud{s} \yLuego j = -1 \implica \paraTodo{j}{(i}{\longitud{s}} \implicaLuego s[j] \neq e) \wedge j \neq -1 \implica (i-1 < j < \longitud{s} \yLuego s[j]=e)) \stackrel{Ax4}{\equiv}$

    $0 \leq i < \longitud{s} \yLuego ( $
    
    $(s[i] = e) \wedge (0 \leq i-1 < \longitud{s} \yLuego i = -1 \implica \paraTodo{i}{(i}{\longitud{s}} \implicaLuego s[i] \neq e) \wedge i \neq -1 \implica (i-1 < i < \longitud{s} \yLuego s[i]=e) ) \vee$

    $(s[i] \neq e) \wedge ( 0 \leq i-1 < \longitud{s} \yLuego j = -1 \implica \paraTodo{j}{(i}{\longitud{s}} \implicaLuego s[j] \neq e) \wedge j \neq -1 \implica (i-1 < j < \longitud{s} \yLuego s[j]=e)))$ \\

    $0 \leq i < \longitud{s} \yLuego j = -1 \implica \paraTodo{j}{(i+1}{\longitud{s}} \implicaLuego s[j] \neq e) \wedge j \neq -1 \implica (i < j < \longitud{s} \yLuego s[j]=e) \implica$

    $0 \leq i < \longitud{s} \yLuego ( $
    
    $(s[i] = e) \implica (i-1 < i < \longitud{s} \yLuego s[i]=e) ) \vee$

    $(s[i] \neq e) \wedge ( 0 \leq i-1 < \longitud{s} \yLuego j = -1 \implica \paraTodo{j}{(i}{\longitud{s}} \implicaLuego s[j] \neq e) \wedge j \neq -1 \implica (i-1 < j < \longitud{s} \yLuego s[j]=e))) \equiv \True$

    \item $\{I \wedge B \wedge (v_{0} = f_{v})\}$ ciclo $\{f_{v} < v_{0}\}$
    
    $wp(i:i-1, i<v_{0}) \equiv i-1<v_{0}$

    $wp(\IfThenElse{s[i]=e}{j:=i}{skip}, i-1) \equiv 0 \leq i < \longitud{s} \yLuego i-1<v_{0}$

    $I \wedge B \wedge v_{0} = i \implica 0 \leq i < \longitud{s} \yLuego i-1<v_{0} \equiv \True$

    \item $(I \wedge f_{v} \leq 0) \implica \neg B$

    $\False \implica i < 0 \equiv \True$
\end{itemize}

\end{document}