## Ejercicio 3

- a) wp(a:= a+1; b:= a/2, b >= 0)
    ~~~
    ≡ Ax3
    ≡ wp(a:= a+1, wp(b:= a/2, b >= 0))
        wp(b:= a/2, b >= 0)
        ≡ Ax1
        ≡ { def(a/2) ∧L a/2 >= 0 }
        ≡ { True ∧L a >= 0 }
        ≡ { a >= 0 }
    ≡ wp(a:= a+1, { a >= 0 })
    ≡ Ax1
    ≡ { def(a+1) ∧L (a >= -1)}
    ≡ { a >= -1 }
    ~~~

- b) wp(a:= A[i] + 1; b:= a*a, b != 2)
    ~~~
    ≡ Ax3
    ≡ wp(a:=A[i]+1, wp(b:= a*a, b != 2))
        ≡ wp(b:= a*a, b != 2)
        ≡ Ax1
        ≡ { def(a*a) ∧L (a*a != 2) }
        ≡ { True ∧L (a*a != 2) }
        ≡ { a*a != 2 }
    ≡ wp(a:=A[i]+1, { a*a != 2 })
    ≡ Ax1
    ≡ { def(A[i] + 1) ∧L ((A[i]+1)*(A[i]+1) != 2) }
    ≡ { 0 <= i < |A| ∧L ((A[i]+1)*(A[i]+1) != 2) }
    ≡ { 0 <= i < |A| ∧L (A[i]*A[i] + 2*A[i] + 1 != 2) }
    ≡ { 0 <= i < |A| ∧L (|A[i]| != 1+sqrt(2)) }
    ~~~

- c) wp(a:= A[i] + 1; a:= b*b, a >= 0)
    ~~~
    ≡ Ax3
        ≡ wp(a:=A[i]+1, wp(a:= b*b, a >= 0))
        ≡ { def(b*b) ∧L (b*b >= 0) }
        ≡ { b*b >= 0 }
    ≡ wp(a:= A[i] + 1; { b*b >= 0 })
    ≡ Ax1
    ≡ { def(A[i] + 1) ∧L (b*b >= 0 })
    ≡ { 0 <= i <= |A| ∧L True }
    ≡ { 0 <= i <= |A| }
    ~~~

- d) wp(a:= a-b; b:= a+b, a >= 0 ∧ b >= 0)
    ~~~
    ≡ wp(a:= a-b; b:= a+b, a >= 0 ∧ b >= 0)
    ≡ Ax3
    ≡ wp(a:= a-b, wp(b:= a+b, a >= 0 ∧ b >= 0))
        ≡ wp(b:= a+b, a >= 0 ∧ b >= 0)
        ≡ { def(a+b) ∧L (a >= 0 ∧ a+b >= 0) }
        ≡ { True ∧L (a >= 0 ∧ a+b >= 0) }
        ≡ { a >= 0 ∧ a+b >= 0 }
    ≡ { def(a-b) ∧ (a-b >= 0 ∧ a-b+b >= 0)}
    ≡ { True ∧ (a-b >= 0 ∧ a >= 0)}
    ≡ { a >= b  ∧ a >= 0)}
    ~~~