\documentclass{article}
\usepackage{xcolor}
\input{../../../../recursos/latex/Algo1Macros.tex}

\begin{document}

\section*{Ejercicio 13}

\subsection*{Correctitud}
\begin{itemize}
    \item $Pre \implica wp($codigo previo al ciclo$, P_{c})$
    \item $P_{c} \implica wp(ciclo, Q_{c})$
    \item $Q_{c} \implica wp($codigo posterior al ciclo$, Post)$
\end{itemize}

Por monotonía sabemos que Pre \implica wp(programa completo, Post)

\subsection*{Teorema del invariante}
\begin{itemize}
    \item $P_{c} \implica I$
    \item $(I \wedge \neg B) \implica Q_{c}$
    \item $\{I \wedge B\}$ ciclo $\{ I \}$
    \item $\{I \wedge B \wedge (v_{0} = f_{v})\}$ ciclo $\{f_{v} < v_{0}\}$
    \item $(I \wedge f_{v} \leq 0) \implica \neg B$
\end{itemize}

\subsection*{Demostración}

\subsubsection*{Datos}
\begin{itemize}
    \item $Pre      \equiv \True$
    \item $Post     \equiv r = \True \Iff \paraTodo{i}{0}{\longitud{s}} \implicaLuego s[i]=s[\longitud{s}-(i+1)]$
    \item $P_{c}    \equiv i = 0 \wedge j = \longitud{s}-1 \wedge r = \True$
    \item $Q_{c}    \equiv r = \True \Iff \paraTodo{i}{0}{\longitud{s}} \implicaLuego s[i]=s[\longitud{s}-(i+1)]$
    \item $I        \equiv (0 \leq i \leq \longitud{s} \wedge j = \longitud{s}-1-i) \yLuego (r = \True \Iff \paraTodo{k}{0}{i} \implicaLuego s[k]=s[\longitud{s}-(k+1)])$
    \item $B        \equiv i < \longitud{s}$
    \item $S1       \equiv \IfThenElse{s[i] \neq s[j]}{r:=\False}{skip}$
    \item $S2       \equiv i:= i + 1$
    \item $S3       \equiv j:= j - 1$
    \item $ciclo    \equiv S1;S2;S3;$
    \item $f_{v}    \equiv \longitud{s} - i$
\end{itemize}

\subsubsection*{$Pre \implica wp($codigo previo al ciclo$, P_{c})$}

$wp(i:=0, wp(j:\longitud{s}-1, wp(r:= \True, i = 0 \wedge j = \longitud{s}-1 \wedge r = \True))) \equiv$

$ 0 = 0 \wedge \longitud{s} - 1 = \longitud{s} -1 \wedge \True = \True \equiv \True$

$ Pre \implica \True \equiv \True \implica \True $

\subsubsection*{$Q_{c} \implica wp($codigo posterior al ciclo$, Post)$}

$wp($codigo posterior al ciclo$, Post) \equiv$ \\

$r = \True \Iff \paraTodo{i}{0}{\longitud{s}} \implicaLuego s[i]=s[\longitud{s}-(i+1)]$

$Q_{c} \implica wp($codigo posterior al ciclo$, Post) \equiv$ \\

$r = \True \Iff \paraTodo{i}{0}{\longitud{s}} \implicaLuego s[i]=s[\longitud{s}-(i+1)] \implica$

$r = \True \Iff \paraTodo{i}{0}{\longitud{s}} \implicaLuego s[i]=s[\longitud{s}-(i+1)] \equiv \True$

\subsubsection*{$P_{c} \implica wp(ciclo, Q_{c})$}

\begin{itemize}
    \item $P_{c} \implica I$

    $i = 0 \wedge j = \longitud{s}-1 \wedge r = \True \implica$
    $(0 \leq i \leq \longitud{s} \wedge j = \longitud{s}-1-i) \yLuego (r = \True \Iff \paraTodo{k}{0}{i} \implicaLuego s[k]=s[\longitud{s}-(k+1)]) \equiv \True$

    \item $(I \wedge \neg B) \implica Q_{c}$
    
    $(0 \leq i \leq \longitud{s} \wedge j = \longitud{s}-1-i) \yLuego (r = \True \Iff \paraTodo{k}{0}{i} \implicaLuego s[k]=s[\longitud{s}-(k+1)]) \wedge i \geq \longitud{s} \implica$

    $r = \True \Iff \paraTodo{i}{0}{\longitud{s}} \implicaLuego s[i]=s[\longitud{s}-(i+1)] \equiv$ \\

    $(i = \longitud{s} \wedge j = \longitud{s}-1-i) \yLuego (r = \True \Iff \paraTodo{k}{0}{i} \implicaLuego s[k]=s[\longitud{s}-(k+1)]) \implica$

    $r = \True \Iff \paraTodo{i}{0}{\longitud{s}} \implicaLuego s[i]=s[\longitud{s}-(i+1)] \equiv \True$ \\

    \item $\{I \wedge B\}$ ciclo $\{ I \}$
    
    $wp(S1;S2;S3, I) \stackrel{Ax3}{\equiv} wp(S1,wp(S2,wp(S3,I)))$

    \begin{itemize}
        \item $wp(S3, I) \equiv wp(j:= j-1, I)$

        $ \{ (0 \leq i \leq \longitud{s} \wedge j = \longitud{s}-1-i) \yLuego (r = \True \Iff \paraTodo{k}{0}{i} \implicaLuego s[k]=s[\longitud{s}-(k+1)]) \} $

        \item $wp(S2,wp(S3, I))\equiv wp(i:= i+1,wp(S3, I)) \equiv$

        $ \{ (0 \leq i+1 \leq \longitud{s} \wedge j = \longitud{s}-i) \yLuego (r = \True \Iff \paraTodo{k}{0}{i} \implicaLuego s[k]=s[\longitud{s}-(k+1)]) \} $

        \item $wp(S1,wp(S2,wp(S3,I))) \equiv $

        $ wp(\IfThenElse{s[i] \neq s[j]}{r:=\False}{skip},(0 \leq i+1 \leq \longitud{s} \wedge j = \longitud{s}-i)) \yLuego (r = \True \Iff \paraTodo{k}{0}{i} \implicaLuego s[k]=s[\longitud{s}-(k+1)])) \stackrel{Ax4}{\equiv} $

        $ (0 \leq i < \longitud{s} \wedge 0 \leq j < \longitud{s}) \yLuego ($

        $ ( s[i] \neq s[j] \wedge ((0 \leq i+1 \leq \longitud{s} \wedge j = \longitud{s}-i)) \yLuego (\False = \True \Iff \paraTodo{k}{0}{i} \implicaLuego s[k]=s[\longitud{s}-(k+1)]))) \vee$

        $ ( s[i]   =  s[j] \wedge (0 \leq i+1 \leq \longitud{s} \wedge j = \longitud{s}-i)) \yLuego (r = \True \Iff \paraTodo{k}{0}{i} \implicaLuego s[k]=s[\longitud{s}-(k+1)])))$
    \end{itemize}

    $ (0 \leq i \leq \longitud{s} \wedge j = \longitud{s}-1-i) \yLuego (r = \True \Iff \paraTodo{k}{0}{i} \implicaLuego s[k]=s[\longitud{s}-(k+1)]) \wedge s < \longitud{s} \equiv $ \\

    $ (0 \leq i < \longitud{s} \wedge j = \longitud{s}-1-i) \yLuego (r = \True \Iff \paraTodo{k}{0}{i} \implicaLuego s[k]=s[\longitud{s}-(k+1)]) \implica $

    $ (0 \leq i < \longitud{s} \wedge 0 \leq j < \longitud{s}) \yLuego ($

    $ ( s[i] \neq s[j] \wedge (0 \leq i+1 \leq \longitud{s} \wedge j = \longitud{s}-i)) \yLuego (\False = \True \Iff \paraTodo{k}{0}{i} \implicaLuego s[k]=s[\longitud{s}-(k+1)])) \vee$

    $ ( s[i]   =  s[j] \wedge (0 \leq i+1 \leq \longitud{s} \wedge j = \longitud{s}-i)) \yLuego (r = \True \Iff \paraTodo{k}{0}{i} \implicaLuego s[k]=s[\longitud{s}-(k+1)])))\equiv$ \\

    $ (0 \leq i < \longitud{s} \wedge j = \longitud{s}-1-i) \yLuego (r = \True \Iff \paraTodo{k}{0}{i} \implicaLuego s[k]=s[\longitud{s}-(k+1)]) \implica $

    $ (0 \leq i < \longitud{s} \wedge 0 \leq j < \longitud{s}) \yLuego ($

    $ ( s[i]   =  s[j] \wedge (0 \leq i+1 \leq \longitud{s} \wedge j = \longitud{s}-i)) \yLuego (r = \True \Iff \paraTodo{k}{0}{i} \implicaLuego s[k]=s[\longitud{s}-(k+1)])) \equiv \True$

    \item $\{I \wedge B \wedge (v_{0} = f_{v})\}$ ciclo $\{f_{v} < v_{0}\}$
    
    $wp(j:j-1, j<v_{0}) \equiv j-1<v_{0}$

    $wp(i:i+1, j-1<v_{0}) \equiv j-1<v_{0}$

    $wp(\IfThenElse{s[i] \neq s[j]}{r:=\False}{skip}, j-1<v_{0}) \equiv 0 \leq j \longitud{s} \wedge j-1<v_{0}$

    $I \wedge B \wedge v_{0} = j \implica 0 \leq j \longitud{s} \wedge j-1<v_{0} \equiv \True$

    \item $(I \wedge f_{v} \leq 0) \implica \neg B$

    $I \wedge j \leq 0 \implica i < \longitud{s} \equiv \True$
\end{itemize}

\end{document}