\documentclass{article}
\usepackage{xcolor}
\input{../../../../recursos/latex/Algo1Macros.tex}

\begin{document}

\section*{Ejercicio 12}

\subsection*{Correctitud}
\begin{itemize}
    \item $Pre \implica wp($codigo previo al ciclo$, P_{c})$
    \item $P_{c} \implica wp(ciclo, Q_{c})$
    \item $Q_{c} \implica wp($codigo posterior al ciclo$, Post)$
\end{itemize}

Por monotonía sabemos que Pre \implica wp(programa completo, Post)

\subsection*{Teorema del invariante}
\begin{itemize}
    \item $P_{c} \implica I$
    \item $(I \wedge \neg B) \implica Q_{c}$
    \item $\{I \wedge B\}$ ciclo $\{ I \}$
    \item $\{I \wedge B \wedge (v_{0} = f_{v})\}$ ciclo $\{f_{v} < v_{0}\}$
    \item $(I \wedge f_{v} \leq 0) \implica \neg B$
\end{itemize}

\subsection*{Demostración}

\subsubsection*{Datos}
\begin{itemize}
    \item $Pre      \equiv \True$
    \item $Post     \equiv r = \True \Iff \existe{k}{0}{\longitud{s}} \yLuego s[k] = e$
    \item $P_{c}    \equiv i = 0 \wedge j = -1$
    \item $Q_{c}    \equiv j \neq -1 \Iff \existe{k}{0}{\longitud{s}} \yLuego s[k] = e$
    \item $I        \equiv 0 \leq i \leq \longitud{s} \yLuego (j \neq -1 \Iff \existe{k}{0}{i} \yLuego s[k] = e)$
    \item $B        \equiv i < \longitud{s}$
    \item $S1       \equiv \IfThenElse{s[i]=e}{j:=i}{skip}$
    \item $S2       \equiv i:= i + 1$
    \item $ciclo    \equiv S1;S2;$
    \item $f_{v}    \equiv \longitud{s} - i$
\end{itemize}

\subsubsection*{$Pre \implica wp($codigo previo al ciclo$, P_{c})$}

$wp($codigo previo al ciclo$, P_{c}) \equiv$

$wp(i:= 0;j:= -1, j \neq -1 \Iff \existe{k}{0}{\longitud{s}} \yLuego s[k] = e) \stackrel{Ax3}{\equiv}$

$wp(i:= 0, wp(j:= -1, j \neq -1 \Iff \existe{k}{0}{\longitud{s}} \yLuego s[k] = e) $

\begin{itemize}
    \item $wp(j:= -1, j \neq -1 \Iff \existe{k}{0}{\longitud{s}} \yLuego s[k] = e)\stackrel{Ax1}{\equiv}$

    $ \{ -1 \neq -1 \Iff \existe{k}{0}{\longitud{s}} \yLuego s[k] = e \} $
\end{itemize}

$wp(i:= 0, -1 \neq -1 \Iff \existe{k}{0}{\longitud{s}} \yLuego s[k] = e) \stackrel{Ax1}{\equiv}$

$ -1 \neq -1 \Iff \existe{k}{0}{\longitud{s}} \yLuego s[k] = e \equiv \True$

$Pre \implica wp($codigo previo al ciclo$, P_{c})$

$\True \implica \True \equiv \True$

\subsubsection*{$Q_{c} \implica wp($codigo posterior al ciclo$, Post)$}

$wp($codigo posterior al ciclo$, Post) \equiv$ \\

$wp(\IfThenElse{j\neq-1}{r:= \True}{r:= \False}, r = \True \Iff \existe{k}{0}{\longitud{s}} \yLuego s[k] = e) \stackrel{Ax4}{\equiv}$\\

$\{ ((j \neq -1) \wedge (\True = \True \Iff \existe{k}{0}{\longitud{s}} \yLuego s[k] = e)) \vee $

$ ((j = -1) \wedge (\False = \True \Iff \existe{k}{0}{\longitud{s}} \yLuego s[k] = e)) \}$ \\

$Q_{c} \implica wp($codigo posterior al ciclo$, Post) \equiv$ \\

$j \neq -1 \Iff \existe{k}{0}{\longitud{s}} \yLuego s[k] = e \implica$

$((j \neq -1) \wedge (\True = \True \Iff \existe{k}{0}{\longitud{s}} \yLuego s[k] = e)) \vee $

$((j = -1) \wedge (\False = \True \Iff \existe{k}{0}{\longitud{s}} \yLuego s[k] = e)) \equiv \True$

\subsubsection*{$P_{c} \implica wp(ciclo, Q_{c})$}

\begin{itemize}
    \item $P_{c} \implica I$

    $i = 0 \wedge j = -1 \implica$
    $0 \leq i \leq \longitud{s} \yLuego (j \neq -1 \Iff \existe{k}{0}{i} \yLuego s[k] = e) \equiv \True$

    \item $(I \wedge \neg B) \implica Q_{c}$
    
    $0 \leq i \leq \longitud{s} \yLuego (j \neq -1 \Iff \existe{k}{0}{i} \yLuego s[k] = e) \wedge i \geq \longitud{s} \implica$

    $j \neq -1 \Iff \existe{k}{0}{\longitud{s}} \yLuego s[k] = e \equiv$ \\

    $i = \longitud{s} \yLuego (j \neq -1 \Iff \existe{k}{0}{i} \yLuego s[k] = e) \implica$

    $j \neq -1 \Iff \existe{k}{0}{\longitud{s}} \yLuego s[k] = e \equiv$

    \item $\{I \wedge B\}$ ciclo $\{ I \}$
    
    $wp(i:= i+1, 0 \leq i \leq \longitud{s} \yLuego (j \neq -1 \Iff \existe{k}{0}{i} \yLuego s[k] = e))\equiv$

    $0 \leq i+1 \leq \longitud{s} \yLuego (j \neq -1 \Iff \existe{k}{0}{i+1} \yLuego s[k] = e)$

    $wp(\IfThenElse{s[i]=e}{j:=i}{skip},0 \leq i+1 \leq \longitud{s} \yLuego (j \neq -1 \Iff \existe{k}{0}{i+1} \yLuego s[k] = e)) \stackrel{Ax4}{\equiv}$

    $0 \leq i < \longitud{s} \yLuego ( $
    
    $(s[i] = e) \wedge (0 \leq i+1 \leq \longitud{s} \yLuego (i \neq -1 \Iff \existe{k}{0}{i+1} \yLuego s[k] = e)) \vee$

    $(s[i] \neq e) \wedge (0 \leq i+1 \leq \longitud{s} \yLuego (j \neq -1 \Iff \existe{k}{0}{i+1} \yLuego s[k] = e))) \equiv$\\

    $0 \leq i < \longitud{s} \yLuego ( $

    $(s[i] = e) \wedge (i \neq -1 \Iff \existe{k}{0}{i+1} \yLuego s[k] = e) \vee$

    $(s[i] \neq e) \wedge (j \neq -1 \Iff \existe{k}{0}{i+1} \yLuego s[k] = e))$ \\

    $0 \leq i < \longitud{s} \yLuego (j \neq -1 \Iff \existe{k}{0}{i} \yLuego s[k] = e) \implica$

    $0 \leq i < \longitud{s} \yLuego ( $

    $(s[i] = e) \wedge (i \neq -1 \Iff \existe{k}{0}{i+1} \yLuego s[k] = e) \vee$

    $(s[i] \neq e) \wedge (j \neq -1 \Iff \existe{k}{0}{i+1} \yLuego s[k] = e))$ \equiv \True \\

    \item $\{I \wedge B \wedge (v_{0} = f_{v})\}$ ciclo $\{f_{v} < v_{0}\}$
    
    $wp(i:i+1, \longitud{s}-i<v_{0}) \equiv \longitud{s}-i-1<v_{0}$

    $wp(\IfThenElse{s[i]=e}{j:=i}{skip}, \longitud{s}-i-1) \equiv 0 \leq i < \longitud{s} \yLuego \longitud{s}-i-1$

    $I \wedge B \wedge v_{0} = i \implica 0 \leq i < \longitud{s} \yLuego \longitud{s}-i-1 \equiv \True$

    \item $(I \wedge f_{v} \leq 0) \implica \neg B$

    $I \wedge \longitud{s}-i \leq 0 \implica i < \longitud{s} \equiv \True$
\end{itemize}

\end{document}