\documentclass{article}
\input{../../../recursos/latex/Algo1Macros.tex}

\begin{document}

\subsection*{Pregunta 4}
\begin{itemize}
    \item $(I \wedge \neg B) \implica Q_{c}$
    \item $\{I \wedge B\}$ ciclo $\{ I \}$
\end{itemize}

\subsection*{Demostraci√≥n}
\subsubsection*{Datos}
\begin{itemize}
    \item $Q_{c}    \equiv \longitud{s} = \longitud{s_0} \yLuego (\paraTodo{i}{1}{\longitud{s} \yLuego s_0[i-1] < s_0[i] \implicaLuego s[i-1]=s_0[i])  \yLuego $
    
    $(\paraTodo{i}{1}{\longitud{s}} \yLuego s_0[i-1] \geq s_0[i] \implicaLuego s[i-1] = s_0[i-1])}$

    \item $I        \equiv 1 \leq i \leq \longitud{s} \wedge \longitud{s} = \longitud{s_0} \yLuego$

    $(\paraTodo{j}{0}{i-1} \yLuego s_0[j-1] < s_0[j] \implicaLuego s[j-1] = s_0[j]) \wedge $

    $(\paraTodo{j}{0}{i-1} \yLuego s_0[j-1] \geq s_0[j] \implicaLuego s[j-1] = s_0[j-1])$

    $(\paraTodo{j}{i-1}{\longitud{s}} \implicaLuego s[j] = s_0[j])$

    \item $B        \equiv i < \longitud{s}$
    \item $S1       \equiv \IfThenElse{s[i-1] < s[i]}{s[i-1]:= s[i];}{skip;};$
    \item $S2       \equiv i := i + 1$
    \item $ciclo    \equiv S1;S2;$
\end{itemize}

\subsubsection*{$\{I \wedge B\}$ ciclo $\{ I \}$}

$wp(S1;S2, I) \stackrel{Ax3}{\equiv}$

$wp(S1, wp(S2, I))$

\begin{itemize}
    \item $wp(S2; I) \equiv$

    $wp(i := i + 1;, I) \stackrel{Ax1}{\equiv}$

    $\{def(i + 1) \yLuego I_{i+1}^{i})\} \equiv$

    $ \{\True \yLuego 1 \leq i+1 \leq \longitud{s} \wedge \longitud{s} = \longitud{s_0} \yLuego$

    $\quad (\paraTodo{j}{0}{i} \yLuego s_0[j-1] < s_0[j] \implicaLuego s[j-1] = s_0[j])\ \wedge $

    $\quad (\paraTodo{j}{0}{i} \yLuego s_0[j-1] \geq s_0[j] \implicaLuego s[j-1] = s_0[j-1])\ \wedge$

    $\quad (\paraTodo{j}{i}{\longitud{s}} \implicaLuego s[j] = s_0[j])\} \equiv $

    $ $

    $ \{0 \leq i < \longitud{s} \wedge \longitud{s} = \longitud{s_0} \yLuego$

    $\quad (\paraTodo{j}{0}{i} \yLuego s_0[j-1] < s_0[j] \implicaLuego s[j-1] = s_0[j])\ \wedge $

    $\quad (\paraTodo{j}{0}{i} \yLuego s_0[j-1] \geq s_0[j] \implicaLuego s[j-1] = s_0[j-1])\ \wedge$

    $\quad (\paraTodo{j}{i}{\longitud{s}} \implicaLuego s[j] = s_0[j])\} $

    \item $wp(S1, wp(S2, I)) \equiv$

    $ wp(\IfThenElse{s[i-1] < s[i]}{s[i-1]:= s[i];}{skip;};, I_{i+1}^{i}) \stackrel{Ax4}{\equiv}$

    $ $

    $ \{ def(s[i-1] < s[i]) \yLuego ((s[i-1] < s[i] \yLuego wp(s[i-1]:=s[i], I_{i+1}^{i}) \vee $
    $ ( s[i-1] \geq s[i] \yLuego wp(skip;, I_{i+1}^{i}))) \} $

    \begin{itemize}
        \item $def(s[i-1] < s[i]) \equiv 0 \leq i-1 < \longitud{s} \equiv 1 \leq i \leq \longitud{s} $

        \item $wp(skip;, I_{i+1}^{i}) \stackrel{Ax3}{\equiv} I_{i+1}^{i} $

        \item $wp(s[i-1]:=s[i], I_{i+1}^{i}) \stackrel{Ax2}{\equiv} $
        $ wp(s:=setAt(s,i-1, s[i]), I_{i+1}^{i}) \equiv $

        $ $

        $ (((def(s) \wedge def(i-1)) \yLuego 0 \leq i-1 < \longitud{s}) \wedge def(s[i])) \yLuego (I_{i+1}^{i})_{setAt(s,i-1, s[i])}^{s} \equiv $

        $ $

        $ 1 \leq i \leq \longitud{s} \yLuego (I_{i+1}^{i})_{setAt(s,i-1, s[i])}^{s}$

    \end{itemize}

    \item $wp(S1, wp(S2, I)) \equiv$

    $ \Big\{ 1 \leq i \leq \longitud{s}\ \yLuego $ 
    $ \Big( (s[i-1] < s[i] \yLuego 1 \leq i \leq \longitud{s} \yLuego {I_{i+1}^{i}}_{setAt(s,i-1, s[i])}^{s}) \vee $
    $ (s[i-1] \geq s[i] \yLuego I_{i+1}^{i}) \Big) \Big\} \equiv $
 
    $ \Big\{ \Big((1 \leq i \leq \longitud{s} \yLuego s[i-1] < s[i] \yLuego {I_{i+1}^{i}}_{setAt(s,i-1, s[i])}^{s}) \vee $
    $ (1 \leq i \leq \longitud{s}\ \yLuego s[i-1] \geq s[i] \yLuego I_{i+1}^{i}) \Big) \Big\} $

    \begin{itemize}
        
        \item $1 \leq i \leq \longitud{s}\ \yLuego s[i-1] \geq s[i] \yLuego I_{i+1}^{i} \equiv$

        $ $

        $ 1 \leq i \leq \longitud{s}\ \yLuego s[i-1] \geq s[i] \yLuego 0 \leq i < \longitud{s} \wedge \longitud{s} = \longitud{s_0} \yLuego$

        $\quad (\paraTodo{j}{0}{i} \yLuego s_0[j-1] < s_0[j] \implicaLuego s[j-1] = s_0[j])\ \wedge $
    
        $\quad (\paraTodo{j}{0}{i} \yLuego s_0[j-1] \geq s_0[j] \implicaLuego s[j-1] = s_0[j-1])\ \wedge$
    
        $\quad (\paraTodo{j}{i}{\longitud{s}} \implicaLuego s[j] = s_0[j]) \equiv$

        $ $

        $ 1 \leq i < \longitud{s}\ \yLuego s[i-1] \geq s[i] \wedge \longitud{s} = \longitud{s_0}\ \yLuego$

        $\quad (\paraTodo{j}{0}{i} \yLuego s_0[j-1] < s_0[j] \implicaLuego s[j-1] = s_0[j])\ \wedge $
    
        $\quad (\paraTodo{j}{0}{i} \yLuego s_0[j-1] \geq s_0[j] \implicaLuego s[j-1] = s_0[j-1])\ \wedge$
    
        $\quad (\paraTodo{j}{i}{\longitud{s}} \implicaLuego s[j] = s_0[j])$

        $ $

        \item $1 \leq i \leq \longitud{s} \yLuego s[i-1] < s[i] \yLuego {I_{i+1}^{i}}_{setAt(s,i-1, s[i])}^{s} \equiv$

        $ $

        $ 1 \leq i \leq \longitud{s} \yLuego s[i-1] < setAt(s,i-1, s[i])[i]\ \yLuego $

        $ 0 \leq i < \longitud{s} \wedge \longitud{setAt(s,i-1, s[i])} = \longitud{s_0} \yLuego$

        $ \quad (\paraTodo{j}{0}{i} \yLuego s_0[j-1] < s_0[j] \implicaLuego setAt(s,i-1, s[i])[j-1] = s_0[j])\ \wedge $

        $ \quad (\paraTodo{j}{0}{i} \yLuego s_0[j-1] \geq s_0[j] \implicaLuego setAt(s,i-1, s[i])[j-1] = s_0[j-1])\ \wedge$

        $ \quad (\paraTodo{j}{i}{\longitud{setAt(s,i-1, s[i])}} \implicaLuego s[j] = s_0[j]) \equiv$

        $ $

        $ 1 \leq i < \longitud{s} \yLuego s[i-1] < s[i]\ \yLuego \longitud{s} = \longitud{s_0}\ \yLuego $

        $ \quad (\paraTodo{j}{0}{i} \yLuego s_0[j-1] < s_0[j] \implicaLuego setAt(s,i-1, s[i])[j-1] = s_0[j])\ \wedge $

        $ \quad (\paraTodo{j}{0}{i} \yLuego s_0[j-1] \geq s_0[j] \implicaLuego setAt(s,i-1, s[i])[j-1] = s_0[j-1])\ \wedge$

        $ \quad (\paraTodo{j}{i}{\longitud{setAt(s,i-1, s[i])}} \implicaLuego s[j] = s_0[j]) $

    \end{itemize} %%%%%%%%%%

    \item $wp(S1, wp(S2, I)) \equiv$

    $ $

    $ \Big\{ \Big((1 \leq i \leq \longitud{s} \yLuego s[i-1] < s[i] \yLuego {I_{i+1}^{i}}_{setAt(s,i-1, s[i])}^{s}) \vee $
    $ (1 \leq i \leq \longitud{s}\ \yLuego s[i-1] \geq s[i] \yLuego I_{i+1}^{i}) \Big) \Big\} $

    $ $

    $ \Big\{ \Big( $
    $ \big(1 \leq i < \longitud{s} \yLuego s[i-1] < s[i]\ \yLuego \longitud{s} = \longitud{s_0}\ \yLuego $

    $ \quad (\paraTodo{j}{0}{i} \yLuego s_0[j-1] < s_0[j] \implicaLuego setAt(s,i-1, s[i])[j-1] = s_0[j])\ \wedge $

    $ \qquad (\paraTodo{j}{0}{i} \yLuego s_0[j-1] \geq s_0[j] \implicaLuego setAt(s,i-1, s[i])[j-1] = s_0[j-1])\ \wedge$

    $ \qquad (\paraTodo{j}{i}{\longitud{setAt(s,i-1, s[i])}} \implicaLuego setAt(s,i-1, s[i])[j] = s_0[j]) \big) $

    $ \quad \vee $
    
    $ \quad \big( 1 \leq i < \longitud{s}\ \yLuego s[i-1] \geq s[i] \wedge \longitud{s} = \longitud{s_0}\ \yLuego$

    $ \qquad (\paraTodo{j}{0}{i} \yLuego s_0[j-1] < s_0[j] \implicaLuego s[j-1] = s_0[j])\ \wedge $

    $ \qquad (\paraTodo{j}{0}{i} \yLuego s_0[j-1] \geq s_0[j] \implicaLuego s[j-1] = s_0[j-1])\ \wedge$

    $ \qquad (\paraTodo{j}{i}{\longitud{s}} \implicaLuego s[j] = s_0[j]) \big)$
    $ \Big) \Big\} $

\end{itemize}

    \begin{itemize}

        \item QvQ $ I \wedge B \implica wp(ciclo,I)$

        \begin{itemize}
        
            \item $I \wedge B \equiv$
        
        $1 \leq i \leq \longitud{s} \wedge \longitud{s} = \longitud{s_0} \yLuego$

        $(\paraTodo{j}{0}{i-1} \yLuego s_0[j-1] < s_0[j] \implicaLuego s[j-1] = s_0[j]) \wedge $

        $(\paraTodo{j}{0}{i-1} \yLuego s_0[j-1] \geq s_0[j] \implicaLuego s[j-1] = s_0[j-1])$

        $(\paraTodo{j}{i-1}{\longitud{s}} \implicaLuego s[j] = s_0[j]) \wedge i < \longitud{s} \equiv $

        $ $ 

        $1 \leq i < \longitud{s} \wedge \longitud{s} = \longitud{s_0} \yLuego$

        $(\paraTodo{j}{0}{i-1} \yLuego s_0[j-1] < s_0[j] \implicaLuego s[j-1] = s_0[j]) \wedge $

        $(\paraTodo{j}{0}{i-1} \yLuego s_0[j-1] \geq s_0[j] \implicaLuego s[j-1] = s_0[j-1])$

        $(\paraTodo{j}{i-1}{\longitud{s}} \implicaLuego s[j] = s_0[j])$

        \end{itemize}

        \item QvQ $ I \wedge B \implica wp(ciclo,I) \equiv $

        $ 1 \leq i < \longitud{s} \wedge \longitud{s} = \longitud{s_0} \yLuego$

        $ (\paraTodo{j}{0}{i-1} \yLuego s_0[j-1] < s_0[j] \implicaLuego s[j-1] = s_0[j]) \wedge $

        $ (\paraTodo{j}{0}{i-1} \yLuego s_0[j-1] \geq s_0[j] \implicaLuego s[j-1] = s_0[j-1]) \wedge$

        $ (\paraTodo{j}{i-1}{\longitud{s}} \implicaLuego s[j] = s_0[j])$

        $ \qquad\qquad \implica$

        $ \Big\{ \Big( $
        $ \big(1 \leq i < \longitud{s} \yLuego s[i-1] < s[i]\ \yLuego \longitud{s} = \longitud{s_0}\ \yLuego $
    
        $ \quad (\paraTodo{j}{0}{i} \yLuego s_0[j-1] < s_0[j] \implicaLuego setAt(s,i-1, s[i])[j-1] = s_0[j])\ \wedge $

        $ \qquad (\paraTodo{j}{0}{i} \yLuego s_0[j-1] \geq s_0[j] \implicaLuego setAt(s,i-1, s[i])[j-1] = s_0[j-1])\ \wedge$

        $ \qquad (\paraTodo{j}{i}{\longitud{setAt(s,i-1, s[i])}} \implicaLuego setAt(s,i-1, s[i])[j] = s_0[j]) \big) $

        $ \quad \vee $

        $ \quad \big( 1 \leq i < \longitud{s}\ \yLuego s[i-1] \geq s[i] \wedge \longitud{s} = \longitud{s_0}\ \yLuego$

        $ \qquad (\paraTodo{j}{0}{i} \yLuego s_0[j-1] < s_0[j] \implicaLuego s[j-1] = s_0[j])\ \wedge $

        $ \qquad (\paraTodo{j}{0}{i} \yLuego s_0[j-1] \geq s_0[j] \implicaLuego s[j-1] = s_0[j-1])\ \wedge$

        $ \qquad (\paraTodo{j}{i}{\longitud{s}} \implicaLuego s[j] = s_0[j]) \big)$
        $ \Big) \Big\}  $

        \paragraph{Por el antecente se sabe que se cumple para todo 0 \leq j < i - 1, hay que ver si se cumple cuando j = i-1}

        \item $j = i - 1$


    \end{itemize}

\end{document}
