\documentclass{article}
\usepackage{xcolor}
\input{../../../../recursos/latex/Algo1Macros.tex}

\begin{document}

\section*{Ejercicio 4}

\subsection*{a)}

\begin{verbatim}
    i:= 1;
    result:= 1;
    while(i < n) do
        i:= i + 1;
        if n mod i = 0 then result:= result + i else 0 fi;
    endwhile
\end{verbatim}

\subsection*{Teorema del invariante}
\begin{itemize}
    \item $P_{c} \implica I$
    \item $(I \wedge \neg B) \implica Q_{c}$
    \item $\{I \wedge B\}$ ciclo $\{ I \}$
    \item $\{I \wedge B \wedge (v_{0} = f_{v})\}$ ciclo $\{f_{v} < v_{0}\}$
    \item $(I \wedge f_{v} \leq 0) \implica \neg B$
\end{itemize}


\subsection*{DemostraciÃ³n}
\subsubsection*{Datos}
\begin{itemize}
    \item $P_{c}    \equiv n \geq 1 \wedge i = 1 \wedge result = 0$
    \item $Q_{c}    \equiv result = \sum_{j=1}^{n} \IfThenElse{n \bmod j = 0}{j}{0}$
    \item $I        \equiv 1 \leq i \leq n \wedge result = \sum_{j=1}^{i} \IfThenElse{n \bmod j = 0}{j}{0}$
    \item $B        \equiv i < n$
    \item $S1       \equiv i := i + 1$
    \item $S2       \equiv \IfThenElse{n \bmod i = 0}{result:= result + i;}{skip;};$
    \item $ciclo    \equiv S1;S2;$
    \item $f_{v}    \equiv n-i$
\end{itemize}

\subsubsection*{$P_{c} \implica I$}

$n \geq 1 \wedge i = 1 \wedge result = 0 \implica$
$P_{c} \implica I \equiv$
$1 \leq i \leq n \wedge result = \sum_{j=1}^{i} \IfThenElse{n \bmod j = 0}{j}{0}$

\begin{itemize}
    \item $n \geq 1 \wedge i = 1 \wedge result = 1 \implica 1 \leq i \leq n \equiv \True$
    \item $n \geq 1 \wedge i = 1 \wedge result = 1 \implica result = \sum_{j=1}^{i} \IfThenElse{n \bmod j = 0}{j}{skip;} \equiv \True$
\end{itemize}

\subsubsection*{$(I \wedge \neg B) \implica Q_{c}$}

$(I \wedge \neg B) \implica Q_{c} \equiv$

$0 \leq i \leq n \wedge result = \sum_{j=1}^{i} \IfThenElse{n \bmod j = 0}{j}{0} \wedge i > n \implica$
$result = \sum_{j=1}^{n} \IfThenElse{n \bmod j = 0}{j}{0} \equiv$

$i = n \wedge result = \sum_{j=1}^{i} \IfThenElse{n \bmod j = 0}{j}{0} \implica$
$result = \sum_{j=1}^{n} \IfThenElse{n \bmod j = 0}{j}{0} \equiv \True$

\subsubsection*{$\{I \wedge B\}$ ciclo $\{ I \}$}

$wp(S1;S2, I) \stackrel{Ax3}{\equiv}$

$wp(S1, wp(S2, I))$

\begin{itemize}
    \item $wp(S2; I) \equiv$

    $wp(\IfThenElse{n \bmod i = 0}{result:= result + i}{skip;};, 1 \leq i \leq n \wedge result = \sum_{j=1}^{i} \IfThenElse{n \bmod j = 0}{j}{0}) \stackrel{Ax4}{\equiv}$

    $\{def(n \bmod i = 0) \yLuego ((n \bmod i = 0) \wedge wp(result:= result + i, 1 \leq i \leq n \wedge result = \sum_{j=1}^{i} \IfThenElse{n \bmod j = 0}{j}{0}) \vee$

    $ (n \bmod i \neq 0 ) \wedge wp(skip;, 1 \leq i \leq n \wedge result = \sum_{j=1}^{i} \IfThenElse{n \bmod j = 0}{j}{0}))\} \stackrel{Ax1,Ax2}{\equiv}$

    $\{(i \neq 0) \yLuego ((n \bmod i = 0) \wedge 1 \leq i \leq n \wedge result + i = \sum_{j=1}^{i} \IfThenElse{n \bmod j = 0}{j}{0} \vee$

    $ (n \bmod i \neq 0 ) \wedge 1 \leq i \leq n \wedge result = \sum_{j=1}^{i} \IfThenElse{n \bmod j = 0}{j}{0})\} \equiv$

    \item $wp(S1, wp(S2, I)) \equiv$

    $wp(i:= i + 1, (i \neq 0) \yLuego ((n \bmod i = 0) \wedge 1 \leq i \leq n \wedge result + i = \sum_{j=1}^{i} \IfThenElse{n \bmod j = 0}{j}{0} \vee$

    $ (n \bmod i \neq 0 ) \wedge 1 \leq i \leq n \wedge result = \sum_{j=1}^{i} \IfThenElse{n \bmod j = 0}{j}{0})) \stackrel{Ax1}{\equiv}$

    $(i+1 \neq 0) \yLuego ((n \bmod i+1 = 0) \wedge 1 \leq i+1 \leq n \wedge result + i+1 = \sum_{j=1}^{i+1} \IfThenElse{n \bmod j = 0}{j}{0} \vee$

    $ (n \bmod i+1 \neq 0 ) \wedge 1 \leq i+1 \leq n \wedge result = \sum_{j=1}^{i+1} \IfThenElse{n \bmod j = 0}{j}{0}))$

\end{itemize}

Qvq $I \wedge B \implica wp(S1;S2, I)$

\begin{itemize}
    \item $I \wedge B \equiv$
    
    $1 \leq i \leq n \wedge result = \sum_{j=1}^{i} \IfThenElse{n \bmod j = 0}{j}{0} \wedge i < n \equiv$

    $1 \leq i < n \wedge result = \sum_{j=1}^{i} \IfThenElse{n \bmod j = 0}{j}{0}$

    \item $I \wedge B \implica wp(S1;S2, I) \equiv$

    $1 \leq i < n \wedge result = \sum_{j=1}^{i} \IfThenElse{n \bmod j = 0}{j}{0} \implica$

    $(i+1 \neq 0) \yLuego ((n \bmod i+1 = 0) \wedge 1 \leq i+1 \leq n \wedge result + i+1 = \sum_{j=1}^{i+1} \IfThenElse{n \bmod j = 0}{j}{0} \vee$

    $ (n \bmod i+1 \neq 0 ) \wedge 1 \leq i+1 \leq n \wedge result = \sum_{j=1}^{i+1} \IfThenElse{n \bmod j = 0}{j}{0}))$

    \item $1 \leq i < n \wedge result = \sum_{j=1}^{i} \IfThenElse{n \bmod j = 0}{j}{0} \implica (i+1 \neq 0) \equiv \True$ 
    
    \item $1 \leq i < n \wedge result = \sum_{j=1}^{i} \IfThenElse{n \bmod j = 0}{j}{0} \implica$
    
    $((n \bmod i+1 = 0) \wedge (1 \leq i+1 \leq n \wedge result + i+1 = \sum_{j=1}^{i+1} \IfThenElse{n \bmod j = 0}{j}{0}) \vee$

    $ (n \bmod i+1 \neq 0 ) \wedge (1 \leq i+1 \leq n \wedge result = \sum_{j=1}^{i+1} \IfThenElse{n \bmod j = 0}{j}{0}))) \equiv \True$
\end{itemize}
    
\subsubsection*{$\{I \wedge B \wedge (v_{0} = f_{v})\}$ ciclo $\{f_{v} < v_{0}\}$}

$wp(S1;S2, n-i<v_{0}) \stackrel{Ax3}{\equiv}$

$wp(S1, wp(S2, n-i<v_{0})) \stackrel{Ax3}{\equiv}$

\begin{itemize}
    \item $wp(S2, n-i<v_{0}) \equiv$
    
    $ wp(\IfThenElse{n \bmod i = 0}{result:= result + i;}{skip;};, n-i-1<v_{0})) \stackrel{Ax4}{\equiv}$

    $\{(i \neq 0) \yLuego ((n \bmod i = 0) \wedge (n-i-1<v_{0}) \vee$

    $ (n \bmod i \neq 0 ) \wedge (n-i-1<v_{0}))\}$

    \item $wp(S1, wp(S2, f_{v} < v_{0})) \equiv$

    $wp(i := i + 1, (i \neq 0) \yLuego ((n \bmod i = 0) \wedge (n-i-1<v_{0}) \vee (n \bmod i \neq 0 ) \wedge (n-i-1<v_{0}))) \stackrel{Ax1}{\equiv}$

    $\{(i + 1 \neq 0) \yLuego ((n \bmod i + 1 = 0) \wedge (n-i-2<v_{0}) \vee (n \bmod i+1 \neq 0 ) \wedge (n-i-2<v_{0}))\}$

\end{itemize}

Qvq $(I \wedge B \wedge (v_{0} = f_{v})) \implica wp(S1;S2, f_{v} < v_{0})$

$(I \wedge B \wedge (v_{0} = f_{v})) \implica wp(S1;S2, f_{v} < v_{0}) \equiv$

$1 \leq i < n \wedge result = \sum_{j=1}^{i} \IfThenElse{n \bmod j = 0}{j}{0} \wedge (v_{0} = n-i)\implica$

$(i + 1 \neq 0) \yLuego ((n \bmod i + 1 = 0) \wedge (n-i-2<v_{0}) \vee (n \bmod i+1 \neq 0 ) \wedge (n-i-2<v_{0}))$

\subsubsection*{$(I \wedge f_{v} \leq 0) \implica \neg B$}

$(I \wedge f_{v} \leq 0) \implica \neg B \equiv $

$1 \leq i \leq n \wedge result = \sum_{j=1}^{i} \IfThenElse{n \bmod j = 0}{j}{0} \wedge n-i \leq 0 \implica i \geq n$

$1 \leq i \leq n \wedge result = \sum_{j=1}^{i} \IfThenElse{n \bmod j = 0}{j}{0} \wedge n \leq i \implica i \geq n$

$1 \leq i \leq n \wedge result = \sum_{j=1}^{i} \IfThenElse{n \bmod j = 0}{j}{0} \wedge n \leq i \implica i \geq n\Iff$

$n = i \wedge result = \sum_{j=1}^{i} \IfThenElse{n \bmod j = 0}{j}{0} \implica i \geq n \equiv \True$

\end{document}