\documentclass{article}
\usepackage{xcolor}
\input{../../../../recursos/latex/Algo1Macros.tex}

\begin{document}

\section*{Ejercicio 7}

\subsection*{a)}

\begin{verbatim}
    i:= 0;
    while(i < s.size()) do
        r[i] := s[i];
        i := i + 1;
    endwhile
    
\end{verbatim}
\subsection*{Teorema del invariante}
\begin{itemize}
    \item $P_{c} \implica I$
    \item $(I \wedge \neg B) \implica Q_{c}$
    \item $\{I \wedge B\}$ ciclo $\{ I \}$
    \item $\{I \wedge B \wedge (v_{0} = f_{v})\}$ ciclo $\{f_{v} < v_{0}\}$
    \item $(I \wedge f_{v} \leq 0) \implica \neg B$
\end{itemize}

\subsection*{DemostraciÃ³n}
\subsubsection*{Datos}
\begin{itemize}
    \item $P_{c}    \equiv \longitud{s} = \longitud{r} \wedge r = r_{0} \wedge i = 0$
    \item $Q_{c}    \equiv \longitud{s} = \longitud{r} \yLuego \paraTodo{j}{0}{\longitud{s}} \implicaLuego s[j] = r[j]$
    \item $I        \equiv ((0 \leq i \leq \longitud{s}) \wedge (\longitud{s} = \longitud{r})) \yLuego \paraTodo{j}{0}{i} \implicaLuego r[j] = s[j]$
    \item $B        \equiv i < \longitud{s}$
    \item $S1       \equiv r[i]:= s[i]$
    \item $S2       \equiv i:= i + 1;$
    \item $ciclo    \equiv S1;S2;$
    \item $f_{v}    \equiv \longitud{s}-i$
\end{itemize}

\subsubsection*{$P_{c} \implica I$}

$P_{c} \implica I \equiv$

$\longitud{s} = \longitud{r} \wedge r = r_{0} \wedge i = 0 \implica$
$((0 \leq i \leq \longitud{s}) \wedge (\longitud{s} = \longitud{r})) \yLuego \paraTodo{j}{0}{i} \implicaLuego r[j] = s[j] \equiv \True$

\subsubsection*{$(I \wedge \neg B) \implica Q_{c}$}

$(I \wedge \neg B) \implica Q_{c} \equiv \\$

$((0 \leq i \leq \longitud{s}) \wedge (\longitud{s} = \longitud{r})) \yLuego \paraTodo{j}{0}{i} \implicaLuego r[i] = s[i] \wedge i \geq \longitud{s} \implica$

$\longitud{s} = \longitud{r} \yLuego \paraTodo{j}{0}{\longitud{s}} \implicaLuego s[j] = r[j] \equiv \\$

$(i = \longitud{s}) \wedge (\longitud{s} = \longitud{r})) \yLuego \paraTodo{j}{0}{i} \implicaLuego r[i] = s[i] \implica$

$\longitud{s} = \longitud{r} \yLuego \paraTodo{j}{0}{\longitud{s}} \implicaLuego s[j] = r[j] \equiv \True$

\subsubsection*{$\{I \wedge B\}$ ciclo $\{ I \}$}

$wp(S1;S2, I) \stackrel{Ax3}{\equiv}$

$wp(S1, wp(S2, I))$

\begin{itemize}
    \item $wp(S2; I) \equiv$

    $wp(i:= i+1, ((0 \leq i \leq \longitud{s}) \wedge (\longitud{s} = \longitud{r})) \yLuego \paraTodo{j}{0}{i} \implicaLuego r[j] = s[j]) \stackrel{Ax1}{\equiv}$

    $\{((0 \leq i+1 \leq \longitud{s}) \wedge (\longitud{s} = \longitud{r})) \yLuego \paraTodo{j}{0}{i+1} \implicaLuego r[j] = s[j] \}$

    \item $wp(S1, wp(S2, I)) \equiv$

    $wp(r[i] := s[i];, ((0 \leq i+1 \leq \longitud{s}) \wedge (\longitud{s} = \longitud{r})) \yLuego \paraTodo{j}{0}{i+1} \implicaLuego r[j] = s[j])\stackrel{Ax1}{\equiv}$\\

    $\{ (0 \leq i < \longitud{s} \wedge \longitud{r} = \longitud{s}) \yLuego ($

    $ ((0 \leq i+1 \leq \longitud{s}) \wedge (\longitud{s} = \longitud{setAt(r,i,s[i])})) \yLuego \paraTodo{j}{0}{i+1} \implicaLuego setAt(r,i,s[i])[j] = s[j]) $

\end{itemize}

Qvq $I \wedge B \implica wp(S1;S2, I)$

\begin{itemize}
    \item $I \wedge B \equiv$
    
    $ ((0 \leq i \leq \longitud{s}) \wedge (\longitud{s} = \longitud{r})) \yLuego \paraTodo{j}{0}{i} \implicaLuego r[j] = s[j] \wedge i < \longitud{s} \equiv$

    $ ((0 \leq i < \longitud{s}) \wedge (\longitud{s} = \longitud{r})) \yLuego \paraTodo{j}{0}{i} \implicaLuego r[j] = s[j] $

    \item $I \wedge B \implica wp(S1;S2, I) \equiv$

    $ ((0 \leq i < \longitud{s}) \wedge (\longitud{s} = \longitud{r})) \yLuego \paraTodo{j}{0}{i} \implicaLuego r[j] = s[j] \implica$

    $ ((0 \leq i+1 \leq \longitud{s}) \wedge (\longitud{s} = \longitud{setAt(r,i,s[i])})) \yLuego \paraTodo{j}{0}{i+1} \implicaLuego setAt(r,i,s[i])[j] = s[j]) \equiv \True$
\end{itemize}

\subsubsection*{$\{I \wedge B \wedge (v_{0} = f_{v})\}$ ciclo $\{f_{v} < v_{0}\}$}

$wp(S1;S2, \longitud{s}-i<v_{0}) \stackrel{Ax3}{\equiv}$

$wp(S1, wp(S2, \longitud{s}-i<v_{0})) \stackrel{Ax3}{\equiv}$

\begin{itemize}
    \item $wp(S2, n-i<v_{0}) \equiv$
    
    $ wp(i:= i+1, \longitud{s}-i<v_{0})) \stackrel{Ax1}{\equiv}$

    $\{\longitud{s}-i-1<v_{0}) \}$

    \item $wp(S1, wp(S2, f_{v} < v_{0})) \equiv$

    $wp(r[i]:= s[i], \longitud{s}-i-1<v_{0}) \stackrel{Ax4}{\equiv}$

    $\{ (0 \leq i < \longitud{s} \wedge \longitud{r} = \longitud{s}) \yLuego \longitud{s}-i-1<v_{0} \} $

\end{itemize}

Qvq $(I \wedge B \wedge (v_{0} = f_{v})) \implica wp(S1;S2, f_{v} < v_{0})$ \\

$(I \wedge B \wedge (v_{0} = f_{v})) \implica wp(S1;S2, f_{v} < v_{0}) \equiv$ \\

$(I \wedge B \wedge (v_{0} = \longitud{s}-i)\implica$

$((0 \leq i < \longitud{s} \wedge \longitud{r} = \longitud{s}) \yLuego \longitud{s}-i-1<v_{0} \equiv \True$

\subsubsection*{$(I \wedge f_{v} \leq 0) \implica \neg B$}

$(I \wedge f_{v} \leq 0) \implica \neg B \equiv $

$(I \wedge \longitud{s}-i \leq 0 \implica i \geq \longitud{s} \equiv \True$

\end{document}